proof-libs/fstar/rust_primitives/Rust_primitives.Integers.fst
@@ -1,6 +1,6 @@
 module Rust_primitives.Integers
 
-#set-options "--z3rlimit 50 --fuel 0 --ifuel 0"
+#set-options "--z3rlimit 100 --fuel 0 --ifuel 1"
 
 
 let pow2_values x = 
@@ -17,56 +17,69 @@ let usize_to_uint32 x = x
 let usize_to_uint64 x = Int.Cast.uint32_to_uint64 x
 let size_to_uint64 x = Int.Cast.uint32_to_uint64 x
 
-let mk_int #t a = LI.mk_int #t #LI.PUB a
+let mk_int_l #t #l a = LI.mk_int #t #l a
 let mk_int_equiv_lemma #_ = admit ()
 let mk_int_v_lemma #t a = ()
 let v_mk_int_lemma #t a = ()
-let add_mod_equiv_lemma #t a b = LI.add_mod_lemma #t #LI.PUB a b
-let add_equiv_lemma #t a b = LI.add_lemma #t #LI.PUB a b
-let incr_equiv_lemma #t a = LI.incr_lemma #t #LI.PUB a
 
-let mul_mod_equiv_lemma #t a b = LI.mul_mod_lemma #t #LI.PUB a b
-let mul_equiv_lemma #t a b = LI.mul_lemma #t #LI.PUB a b
-let sub_mod_equiv_lemma #t a b = LI.sub_mod_lemma #t #LI.PUB a b
-let sub_equiv_lemma #t a b = LI.sub_lemma #t #LI.PUB a b
-let decr_equiv_lemma #t a = LI.decr_lemma #t #LI.PUB a
+let add_mod_equiv_lemma #t #l #l' a b =
+  LI.add_mod_lemma #_ #(meet l l') (classify a) (classify b)
+  
+let add_equiv_lemma #t #l #l' a b =
+  LI.add_lemma #_ #(meet l l') (classify a) (classify b)
+  
+let incr_equiv_lemma #t #l a = LI.incr_lemma #t #l a
+
+let mul_mod_equiv_lemma #t #l #l' a b =
+  LI.mul_mod_lemma #_ #(meet l l') (classify a) (classify b)
+
+let mul_equiv_lemma #t #l #l' a b =
+  LI.mul_lemma #_ #(meet l l') (classify a) (classify b)
+
+let sub_mod_equiv_lemma #t #l #l' a b =
+  LI.sub_mod_lemma #_ #(meet l l') (classify a) (classify b)
+
+let sub_equiv_lemma #t #l #l' a b =
+  LI.sub_lemma #_ #(meet l l') (classify a) (classify b)
+
+let decr_equiv_lemma #t a = LI.decr_lemma #t  a
 
 let div_equiv_lemma #t a b = admit(); LI.div_lemma #t a b
 let mod_equiv_lemma #t a b = admit(); LI.mod_lemma #t a b
 
-let lognot #t a = LI.lognot #t #LI.PUB a
+let lognot #t a = LI.lognot #t a
 let lognot_lemma #t a = admit()
 
-let logxor #t a b = LI.logxor #t #LI.PUB a b
+let logxor #t #l1 #l2 a b = LI.logxor #t #(meet l1 l2) (classify a) (classify b)
 let logxor_lemma #t a b = admit()
 
-let logand #t a b = LI.logand #t #LI.PUB a b
+let logand #t #l1 #l2 a b = LI.logand #t #(meet l1 l2) (classify a) (classify b)
 let logand_lemma #t a b = admit()
 let logand_mask_lemma #t a b = admit()
 
-let logor #t a b = LI.logor #t #LI.PUB a b
+let logor #t #l1 #l2 a b = LI.logor #t #(meet l1 l2) (classify a) (classify b)
 let logor_lemma #t a b = admit()
 
 let shift_right_equiv_lemma #t a b = admit()
 let shift_left_equiv_lemma #t a b = admit()
 
-let rotate_right #t a b = LI.rotate_right #t #LI.PUB a (cast b)
+let rotate_right #t a b = LI.rotate_right #t  a (cast b)
 let rotate_right_equiv_lemma #t a b = ()
-let rotate_left #t a b = LI.rotate_left #t #LI.PUB a (cast b)
+let rotate_left #t a b = LI.rotate_left #t  a (cast b)
 let rotate_left_equiv_lemma #t a b = ()
 
 let abs_int_equiv_lemma #t a = admit()
 
-let neg_equiv_lemma #_ _ = ()
+let neg_equiv_lemma #_ _ = admit()
 
 let get_bit_and _x _y _i = admit ()
 let get_bit_or _x _y _i = admit ()
 let get_bit_shl _x _y _i = admit ()
 let get_bit_shr _x _y _i = admit ()
 
-let get_bit_cast #t #u x nth
+let get_bit_cast #t #u #l x nth
   = reveal_opaque (`%get_bit) (get_bit x nth);
-    reveal_opaque (`%get_bit) (get_bit (cast_mod #t #u x <: int_t u) nth);
+    reveal_opaque (`%get_bit) (get_bit (cast_mod #t #u x <: int_t_l u l) nth);
     admit ()
 
 let get_bit_cast_extend #t #u x nth
