proof-libs/fstar/core/Core.Num.fsti
@@ -13,7 +13,7 @@ val impl__u32__from_be_bytes: t_Array u8 (sz 4) -> u32
 val impl__u32__to_le_bytes: u32 -> t_Array u8 (sz 4)
 val impl__u32__to_be_bytes: u32 -> t_Array u8 (sz 4)
 val impl__u32__rotate_right: u32 -> u32 -> u32
-let impl__u32__BITS: u32 = 32ul
+let impl__u32__BITS: u32 = classify (32ul <: pub_int_t u32_inttype)
 
 let impl__u64__wrapping_add: u64 -> u64 -> u64 = add_mod
 val impl__u64__rotate_left: u32 -> u32 -> u32
@@ -23,7 +23,7 @@ val impl__u64__to_le_bytes: u64 -> t_Array u8 (sz 8)
 val impl__u64__to_be_bytes: u64 -> t_Array u8 (sz 8)
 val impl__u64__rotate_right: u64 -> u64 -> u64
 
-let impl__u128__wrapping_add (x: u128) (y: u128): u128 = FStar.UInt128.add_underspec x y
+let impl__u128__wrapping_add (x: u128) (y: u128): u128 = add_mod x y //FStar.UInt128.add_underspec x y
 val impl__u128__rotate_left: u128 -> u128 -> u128
 val impl__u128__from_le_bytes: t_Array u8 (sz 16) -> u128
 val impl__u128__from_be_bytes: t_Array u8 (sz 16) -> u128
