proof-libs/fstar/rust_primitives/Rust_primitives.Hax.fst
@@ -18,14 +18,14 @@ class update_at_tc self idx = {
 
 open Core.Slice
 
-instance impl__index t l n: t_Index (t_Array t l) (int_t n)
+instance impl__index t l n: t_Index (t_Array t l) (pub_int_t n)
   = { f_Output = t;
-      in_range = (fun (s: t_Array t l) (i: int_t n) -> v i >= 0 && v i < v l);
+      in_range = (fun (s: t_Array t l) (i: pub_int_t n) -> v i >= 0 && v i < v l);
       f_index = (fun s i -> Seq.index s (v i));
     }
 
-instance update_at_tc_array t l n: update_at_tc (t_Array t l) (int_t n) = {
-  super_index = FStar.Tactics.Typeclasses.solve <: t_Index (t_Array t l) (int_t n);
+instance update_at_tc_array t l n: update_at_tc (t_Array t l) (pub_int_t n) = {
+  super_index = FStar.Tactics.Typeclasses.solve <: t_Index (t_Array t l) (pub_int_t n);
   update_at = (fun arr i x -> FStar.Seq.upd arr (v i) x);
 }
 
